

CSL302: Compiler Design

Syntax Analysis

Vishwesh Jatala

Assistant Professor

Department of CSE

Indian Institute of Technology Bhilai

vishwesh@iitbhilai.ac.in



Acknowledgement

- Today's slides are modified from that of
 - *Stanford University:*
 - <https://web.stanford.edu/class/archive/cs/cs143/cs143.112>
8/

Predictive Parsing

- The leftmost DFS/BFS algorithms are **backtracking** algorithms.
 - Guess which production to use, then back up if it doesn't work.
 - Try to match a prefix by sheer dumb luck.
- There is another class of parsing algorithms called **predictive** algorithms.
 - Based on remaining input, predict (*without backtracking*) which production to use.

Exploiting Lookahead

- Given just the start symbol, how do you know which productions to use to get to the input program?
- Idea: Use **lookahead tokens**.
- When trying to decide which production to use, look at some number of tokens of the input to help make the decision.

A Simple Predictive Parser: **LL(1)**

- Top-down, predictive parsing:
 - **L**: Left-to-right scan of the tokens
 - **L**: Leftmost derivation.
 - **(1)**: One token of lookahead
- Construct a leftmost derivation for the sequence of tokens.
- When expanding a nonterminal, we predict the production to use by looking at the next token of the input. **The decision is forced.**

Predictive Parsing

$E \rightarrow \text{int}$

$E \rightarrow (E \text{ Op } E)$

$\text{Op} \rightarrow +$

$\text{Op} \rightarrow *$

(int	+	(int	*	int))
---	-----	---	---	-----	---	-----	---	---

Predictive Parsing

E

$E \rightarrow \text{int}$

$E \rightarrow (E \text{ Op } E)$

$\text{Op} \rightarrow +$

$\text{Op} \rightarrow *$

(int	+	(int	*	int))
---	-----	---	---	-----	---	-----	---	---

Predictive Parsing

E
(E Op E)

E \rightarrow **int**

E \rightarrow **(E Op E)**

Op \rightarrow **+**

Op \rightarrow *****

(int	+	(int	*	int))
---	-----	---	---	-----	---	-----	---	---

Predictive Parsing

E
(E Op E)
(int Op E)

E → int

E → (E Op E)

Op → +

Op → *

(int	+	(int	*	int))
---	-----	---	---	-----	---	-----	---	---

Predictive Parsing

E
(E Op E)
(int Op E)
(int + E)

E → int

E → (E Op E)

Op → +

Op → *

(int	+	(int	*	int))
---	-----	---	---	-----	---	-----	---	---

Predictive Parsing

$E \rightarrow \text{int}$

$E \rightarrow (E \text{ Op } E)$

$\text{Op} \rightarrow +$

$\text{Op} \rightarrow *$

E
(E Op E)
(int Op E)
(int + E)
(int + (E Op E))

(int	+	(int	*	int))
---	-----	---	---	-----	---	-----	---	---

Predictive Parsing

$E \rightarrow \text{int}$

$E \rightarrow (E \text{ Op } E)$

$\text{Op} \rightarrow +$

$\text{Op} \rightarrow *$

E
(E Op E)
(int Op E)
(int + E)
(int + (E Op E))
(int + (int Op E))

(int	+	(int	*	int))
---	-----	---	---	-----	---	-----	---	---

Predictive Parsing

$E \rightarrow \text{int}$
 $E \rightarrow (E \text{ Op } E)$
 $\text{Op} \rightarrow +$
 $\text{Op} \rightarrow *$

E
(E Op E)
(int Op E)
(int + E)
(int + (E Op E))
(int + (int Op E))
(int + (int * E))

(int	+	(int	*	int))
---	-----	---	---	-----	---	-----	---	---

Predictive Parsing

$E \rightarrow \text{int}$

$E \rightarrow (E \text{ Op } E)$

$\text{Op} \rightarrow +$

$\text{Op} \rightarrow *$

E
(E Op E)
(int Op E)
(int + E)
(int + (E Op E))
(int + (int Op E))
(int + (int * E))
(int + (int * int))

(int	+	(int	*	int))
---	-----	---	---	-----	---	-----	---	---

Predictive Parsing

$E \rightarrow \text{int}$
 $E \rightarrow (E \text{ Op } E)$
 $\text{Op} \rightarrow +$
 $\text{Op} \rightarrow *$

E
(E Op E)
(int Op E)
(int + E)
(int + (E Op E))
(int + (int Op E))
(int + (int * E))
(int + (int * int))

(int	+	(int	*	int))
---	-----	---	---	-----	---	-----	---	---

LL(1) Parse Tables

$E \rightarrow \text{int}$

$E \rightarrow (E \text{ Op } E)$

$\text{Op} \rightarrow +$

$\text{Op} \rightarrow *$

LL(1) Parse Tables

$E \rightarrow \text{int}$

$E \rightarrow (E \text{ Op } E)$

$\text{Op} \rightarrow +$

$\text{Op} \rightarrow *$

	int	()	+	*
E	int	(E Op E)			
Op				+	*

LL(1) Parsing

(int + (int * int))

- (1) $E \rightarrow \text{int}$
- (2) $E \rightarrow (E \text{ Op } E)$
- (3) $\text{Op} \rightarrow +$
- (4) $\text{Op} \rightarrow *$

LL(1) Parsing

E	(int + (int * int))
---	---------------------

- (1) $E \rightarrow \text{int}$
- (2) $E \rightarrow (E \text{ Op } E)$
- (3) $\text{Op} \rightarrow +$
- (4) $\text{Op} \rightarrow *$

LL(1) Parsing

E	(int + (int * int))
---	---------------------

- (1) $E \rightarrow \text{int}$
- (2) $E \rightarrow (E \text{ Op } E)$
- (3) $\text{Op} \rightarrow +$
- (4) $\text{Op} \rightarrow *$

	int	()	+	*
E	1	2			
Op				3	4

LL(1) Parsing

E\$	(int + (int * int))\$
-----	-----------------------

- (1) $E \rightarrow \text{int}$
- (2) $E \rightarrow (E \text{ Op } E)$
- (3) $\text{Op} \rightarrow +$
- (4) $\text{Op} \rightarrow *$

	int	()	+	*
E	1	2			
Op				3	4

LL(1) Parsing

E\$	(int + (int * int))\$
-----	-----------------------

- (1) $E \rightarrow \text{int}$
- (2) $E \rightarrow (E \text{ Op } E)$
- (3) $\text{Op} \rightarrow +$
- (4) $\text{Op} \rightarrow *$

	int	()	+	*
E	1	2			
Op				3	4

The \$ symbol is the end-of-input marker and is used by the parser to detect when we have reached the end of the input. It is not a part of the grammar.

LL(1) Parsing

E\$	(int + (int * int))\$
-----	-----------------------

- (1) $E \rightarrow \text{int}$
- (2) $E \rightarrow (E \text{ Op } E)$
- (3) $\text{Op} \rightarrow +$
- (4) $\text{Op} \rightarrow *$

	int	()	+	*
E	1	2			
Op				3	4

LL(1) Parsing

E\$	(int + (int * int))\$
-----	-----------------------

- (1) **E** \rightarrow **int**
- (2) **E** \rightarrow **(E Op E)**
- (3) **Op** \rightarrow **+**
- (4) **Op** \rightarrow *****

	int	()	+	*
E	1	2			
Op				3	4

LL(1) Parsing

E\$	(int + (int * int))\$
-----	-----------------------

- (1) $E \rightarrow \text{int}$
- (2) $E \rightarrow (E \text{ Op } E)$
- (3) $\text{Op} \rightarrow +$
- (4) $\text{Op} \rightarrow *$

	int	()	+	*
E	1	2			
Op				3	4

LL(1) Parsing

- (1) $E \rightarrow \text{int}$
- (2) $E \rightarrow (E \text{ Op } E)$
- (3) $\text{Op} \rightarrow +$
- (4) $\text{Op} \rightarrow *$

$E\$$	$(\text{int} + (\text{int} * \text{int}))\$$
$(E \text{ Op } E) \$$	$(\text{int} + (\text{int} * \text{int}))\$$

	int	()	+	*
E	1	2			
Op				3	4

LL(1) Parsing

- (1) $E \rightarrow \text{int}$
- (2) $E \rightarrow (E \text{ Op } E)$
- (3) $\text{Op} \rightarrow +$
- (4) $\text{Op} \rightarrow *$

$E\$$	$(\text{int} + (\text{int} * \text{int}))\$$
$(E \text{ Op } E) \$$	$(\text{int} + (\text{int} * \text{int}))\$$

The first symbol of our guess is now a terminal symbol. We thus match it against the first symbol of the string to parse.

This is called a match step.

	int	()	+	*
E	1	2			
Op				3	4

LL(1) Parsing

- (1) $E \rightarrow \text{int}$
- (2) $E \rightarrow (E \text{ Op } E)$
- (3) $\text{Op} \rightarrow +$
- (4) $\text{Op} \rightarrow *$

$E\$$	$(\text{int} + (\text{int} * \text{int}))\$$
$(E \text{ Op } E) \$$	$(\text{int} + (\text{int} * \text{int}))\$$
$E \text{ Op } E) \$$	$\text{int} + (\text{int} * \text{int}))\$$

	int	()	+	*
E	1	2			
Op				3	4

LL(1) Parsing

- (1) $E \rightarrow \text{int}$
- (2) $E \rightarrow (E \text{ Op } E)$
- (3) $\text{Op} \rightarrow +$
- (4) $\text{Op} \rightarrow *$

$E\$$	$(\text{int} + (\text{int} * \text{int}))\$$
$(E \text{ Op } E) \$$	$(\text{int} + (\text{int} * \text{int}))\$$
$E \text{ Op } E) \$$	$\text{int} + (\text{int} * \text{int}))\$$

	int	()	+	*
E	1	2			
Op				3	4

LL(1) Parsing

- (1) **E** \rightarrow **int**
- (2) **E** \rightarrow **(E Op E)**
- (3) **Op** \rightarrow **+**
- (4) **Op** \rightarrow *****

E\$	(int + (int * int))\$
(E Op E) \$	(int + (int * int))\$
E Op E) \$	int + (int * int))\$
int Op E) \$	int + (int * int))\$

	int	()	+	*
E	1	2			
Op				3	4

LL(1) Parsing

- (1) **E** \rightarrow **int**
 (2) **E** \rightarrow **(E Op E)**
 (3) **Op** \rightarrow **+**
 (4) **Op** \rightarrow *****

E\$	(int + (int * int))\$
(E Op E) \$	(int + (int * int))\$
E Op E) \$	int + (int * int))\$
int Op E) \$	int + (int * int))\$
Op E) \$	+ (int * int))\$

	int	()	+	*
E	1	2			
Op				3	4

LL(1) Parsing

- (1) **E** \rightarrow **int**
- (2) **E** \rightarrow **(E Op E)**
- (3) **Op** \rightarrow **+**
- (4) **Op** \rightarrow *****

E\$	(int + (int * int))\$
(E Op E) \$	(int + (int * int))\$
E Op E) \$	int + (int * int))\$
int Op E) \$	int + (int * int))\$
Op E) \$	+ (int * int))\$

	int	()	+	*
E	1	2			
Op				3	4

LL(1) Parsing

- (1) **E** \rightarrow **int**
 (2) **E** \rightarrow **(E Op E)**
 (3) **Op** \rightarrow **+**
 (4) **Op** \rightarrow *****

E\$	(int + (int * int))\$
(E Op E) \$	(int + (int * int))\$
E Op E) \$	int + (int * int))\$
int Op E) \$	int + (int * int))\$
Op E) \$	+ (int * int))\$
+ E) \$	+ (int * int))\$

	int	()	+	*
E	1	2			
Op				3	4

LL(1) Parsing

- (1) **E** \rightarrow **int**
 (2) **E** \rightarrow **(E Op E)**
 (3) **Op** \rightarrow **+**
 (4) **Op** \rightarrow *****

E\$	(int + (int * int))\$
(E Op E) \$	(int + (int * int))\$
E Op E) \$	int + (int * int))\$
int Op E) \$	int + (int * int))\$
Op E) \$	+ (int * int))\$
+ E) \$	+ (int * int))\$
E) \$	(int * int))\$

	int	()	+	*
E	1	2			
Op				3	4

LL(1) Parsing

- (1) **E** \rightarrow **int**
 (2) **E** \rightarrow **(E Op E)**
 (3) **Op** \rightarrow **+**
 (4) **Op** \rightarrow *****

E\$	(int + (int * int))\$
(E Op E) \$	(int + (int * int))\$
E Op E) \$	int + (int * int))\$
int Op E) \$	int + (int * int))\$
Op E) \$	+ (int * int))\$
+ E) \$	+ (int * int))\$
E) \$	(int * int))\$

	int	()	+	*
E	1	2			
Op				3	4

LL(1) Parsing

- (1) **E** \rightarrow **int**
 (2) **E** \rightarrow **(E Op E)**
 (3) **Op** \rightarrow **+**
 (4) **Op** \rightarrow *****

	int	()	+	*
E	1	2			
Op				3	4

E\$	(int + (int * int))\$
(E Op E) \$	(int + (int * int))\$
E Op E) \$	int + (int * int))\$
int Op E) \$	int + (int * int))\$
Op E) \$	+ (int * int))\$
+ E) \$	+ (int * int))\$
E) \$	(int * int))\$
(E Op E)) \$	(int * int))\$

LL(1) Parsing

- (1) **E** \rightarrow **int**
 (2) **E** \rightarrow **(E Op E)**
 (3) **Op** \rightarrow **+**
 (4) **Op** \rightarrow *****

	int	()	+	*
E	1	2			
Op				3	4

E\$	(int + (int * int))\$
(E Op E) \$	(int + (int * int))\$
E Op E) \$	int + (int * int))\$
int Op E) \$	int + (int * int))\$
Op E) \$	+ (int * int))\$
+ E) \$	+ (int * int))\$
E) \$	(int * int))\$
(E Op E)) \$	(int * int))\$
E Op E)) \$	int * int))\$

LL(1) Parsing

- (1) **E** \rightarrow **int**
 (2) **E** \rightarrow **(E Op E)**
 (3) **Op** \rightarrow **+**
 (4) **Op** \rightarrow *****

	int	()	+	*
E	1	2			
Op				3	4

E\$	(int + (int * int))\$
(E Op E) \$	(int + (int * int))\$
E Op E) \$	int + (int * int))\$
int Op E) \$	int + (int * int))\$
Op E) \$	+ (int * int))\$
+ E) \$	+ (int * int))\$
E) \$	(int * int))\$
(E Op E)) \$	(int * int))\$
E Op E)) \$	int * int))\$

LL(1) Parsing

- (1) **E** \rightarrow **int**
 (2) **E** \rightarrow **(E Op E)**
 (3) **Op** \rightarrow **+**
 (4) **Op** \rightarrow *****

	int	()	+	*
E	1	2			
Op				3	4

E\$	(int + (int * int))\$
(E Op E) \$	(int + (int * int))\$
E Op E) \$	int + (int * int))\$
int Op E) \$	int + (int * int))\$
Op E) \$	+ (int * int))\$
+ E) \$	+ (int * int))\$
E) \$	(int * int))\$
(E Op E)) \$	(int * int))\$
E Op E)) \$	int * int))\$
int Op E)) \$	int * int))\$

int)) \$

LL(1) Parsing

- (1) **E** \rightarrow **int**
 (2) **E** \rightarrow **(E Op E)**
 (3) **Op** \rightarrow **+**
 (4) **Op** \rightarrow *****

	int	()	+	*
E	1	2			
Op				3	4

E\$	(int + (int * int))\$
(E Op E) \$	(int + (int * int))\$
E Op E) \$	int + (int * int))\$
int Op E) \$	int + (int * int))\$
Op E) \$	+ (int * int))\$
+ E) \$	+ (int * int))\$
E) \$	(int * int))\$
(E Op E)) \$	(int * int))\$
E Op E)) \$	int * int))\$
int Op E)) \$	int * int))\$
Op E)) \$	* int))\$

LL(1) Parsing

- (1) **E** \rightarrow **int**
 (2) **E** \rightarrow **(E Op E)**
 (3) **Op** \rightarrow **+**
 (4) **Op** \rightarrow *****

	int	()	+	*
E	1	2			
Op				3	4

E\$	(int + (int * int))\$
(E Op E) \$	(int + (int * int))\$
E Op E) \$	int + (int * int))\$
int Op E) \$	int + (int * int))\$
Op E) \$	+ (int * int))\$
+ E) \$	+ (int * int))\$
E) \$	(int * int))\$
(E Op E)) \$	(int * int))\$
E Op E)) \$	int * int))\$
int Op E)) \$	int * int))\$
Op E)) \$	* int))\$

LL(1) Parsing

- (1) **E** \rightarrow **int**
 (2) **E** \rightarrow **(E Op E)**
 (3) **Op** \rightarrow **+**
 (4) **Op** \rightarrow *****

	int	()	+	*
E	1	2			
Op				3	4

E\$	(int + (int * int))\$
(E Op E) \$	(int + (int * int))\$
E Op E) \$	int + (int * int))\$
int Op E) \$	int + (int * int))\$
Op E) \$	+ (int * int))\$
+ E) \$	+ (int * int))\$
E) \$	(int * int))\$
(E Op E)) \$	(int * int))\$
E Op E)) \$	int * int))\$
int Op E)) \$	int * int))\$
Op E)) \$	* int))\$
* E)) \$	* int))\$

LL(1) Parsing

- (1) **E** \rightarrow **int**
 (2) **E** \rightarrow **(E Op E)**
 (3) **Op** \rightarrow **+**
 (4) **Op** \rightarrow *****

	int	()	+	*
E	1	2			
Op				3	4

E\$	(int + (int * int))\$
(E Op E) \$	(int + (int * int))\$
E Op E) \$	int + (int * int))\$
int Op E) \$	int + (int * int))\$
Op E) \$	+ (int * int))\$
+ E) \$	+ (int * int))\$
E) \$	(int * int))\$
(E Op E)) \$	(int * int))\$
E Op E)) \$	int * int))\$
int Op E)) \$	int * int))\$
Op E)) \$	* int))\$
* E)) \$	* int))\$
E)) \$	int))\$

LL(1) Parsing

- (1) **E** \rightarrow **int**
 (2) **E** \rightarrow **(E Op E)**
 (3) **Op** \rightarrow **+**
 (4) **Op** \rightarrow *****

	int	()	+	*
E	1	2			
Op				3	4

E\$	(int + (int * int))\$
(E Op E) \$	(int + (int * int))\$
E Op E) \$	int + (int * int))\$
int Op E) \$	int + (int * int))\$
Op E) \$	+ (int * int))\$
+ E) \$	+ (int * int))\$
E) \$	(int * int))\$
(E Op E)) \$	(int * int))\$
E Op E)) \$	int * int))\$
int Op E)) \$	int * int))\$
Op E)) \$	* int))\$
* E)) \$	* int))\$
E)) \$	int))\$

LL(1) Parsing

- (1) **E** \rightarrow **int**
 (2) **E** \rightarrow **(E Op E)**
 (3) **Op** \rightarrow **+**
 (4) **Op** \rightarrow *****

	int	()	+	*
E	1	2			
Op				3	4

E\$	(int + (int * int))\$
(E Op E) \$	(int + (int * int))\$
E Op E) \$	int + (int * int))\$
int Op E) \$	int + (int * int))\$
Op E) \$	+ (int * int))\$
+ E) \$	+ (int * int))\$
E) \$	(int * int))\$
(E Op E)) \$	(int * int))\$
E Op E)) \$	int * int))\$
int Op E)) \$	int * int))\$
Op E)) \$	* int))\$
* E)) \$	* int))\$
E)) \$	int))\$
int)) \$	int))\$

LL(1) Parsing

- (1) **E** \rightarrow **int**
 (2) **E** \rightarrow **(E Op E)**
 (3) **Op** \rightarrow **+**
 (4) **Op** \rightarrow *****

	int	()	+	*
E	1	2			
Op				3	4

E\$	(int + (int * int))\$
(E Op E) \$	(int + (int * int))\$
E Op E) \$	int + (int * int))\$
int Op E) \$	int + (int * int))\$
Op E) \$	+ (int * int))\$
+ E) \$	+ (int * int))\$
E) \$	(int * int))\$
(E Op E)) \$	(int * int))\$
E Op E)) \$	int * int))\$
int Op E)) \$	int * int))\$
Op E)) \$	* int))\$
* E)) \$	* int))\$
E)) \$	int))\$
int)) \$	int))\$
)) \$))\$

LL(1) Parsing

- (1) **E** \rightarrow **int**
 (2) **E** \rightarrow **(E Op E)**
 (3) **Op** \rightarrow **+**
 (4) **Op** \rightarrow *****

	int	()	+	*
E	1	2			
Op				3	4

E\$	(int + (int * int))\$
(E Op E) \$	(int + (int * int))\$
E Op E) \$	int + (int * int))\$
int Op E) \$	int + (int * int))\$
Op E) \$	+ (int * int))\$
+ E) \$	+ (int * int))\$
E) \$	(int * int))\$
(E Op E)) \$	(int * int))\$
E Op E)) \$	int * int))\$
int Op E)) \$	int * int))\$
Op E)) \$	* int))\$
* E)) \$	* int))\$
E)) \$	int))\$
int)) \$	int))\$
)) \$))\$
) \$)\$

LL(1) Parsing

- (1) **E** \rightarrow **int**
 (2) **E** \rightarrow **(E Op E)**
 (3) **Op** \rightarrow **+**
 (4) **Op** \rightarrow *****

	int	()	+	*
E	1	2			
Op				3	4

E\$	(int + (int * int))\$
(E Op E) \$	(int + (int * int))\$
E Op E) \$	int + (int * int))\$
int Op E) \$	int + (int * int))\$
Op E) \$	+ (int * int))\$
+ E) \$	+ (int * int))\$
E) \$	(int * int))\$
(E Op E)) \$	(int * int))\$
E Op E)) \$	int * int))\$
int Op E)) \$	int * int))\$
Op E)) \$	* int))\$
* E)) \$	* int))\$
E)) \$	int))\$
int)) \$	int))\$
)) \$))\$
) \$)\$
\$	\$

LL(1) Error Detection

- (1) $E \rightarrow \text{int}$
- (2) $E \rightarrow (E \text{ Op } E)$
- (3) $\text{Op} \rightarrow +$
- (4) $\text{Op} \rightarrow *$

int + int\$

	int	()	+	*
E	1	2			
Op				3	4

LL(1) Error Detection

- (1) **E** \rightarrow **int**
- (2) **E** \rightarrow (**E Op E**)
- (3) **Op** \rightarrow **+**
- (4) **Op** \rightarrow *****

E\$	int + int\$
-----	-------------

	int	()	+	*
E	1	2			
Op				3	4

LL(1) Error Detection

- (1) **E** \rightarrow **int**
- (2) **E** \rightarrow **(E Op E)**
- (3) **Op** \rightarrow **+**
- (4) **Op** \rightarrow *****

E\$	int + int\$
-----	-------------

	int	()	+	*
E	1	2			
Op				3	4

LL(1) Error Detection

- (1) **E** \rightarrow **int**
- (2) **E** \rightarrow (**E Op E**)
- (3) **Op** \rightarrow **+**
- (4) **Op** \rightarrow *****

E\$	int + int\$
int \$	int + int\$

	int	()	+	*
E	1	2			
Op				3	4

LL(1) Error Detection

- (1) **E** \rightarrow **int**
- (2) **E** \rightarrow **(E Op E)**
- (3) **Op** \rightarrow **+**
- (4) **Op** \rightarrow *****

E\$	int + int\$
int \$	int + int\$
\$	+ int\$

	int	()	+	*
E	1	2			
Op				3	4

LL(1) Error Detection

- (1) **E** \rightarrow **int**
- (2) **E** \rightarrow (**E Op E**)
- (3) **Op** \rightarrow **+**
- (4) **Op** \rightarrow *****

E\$	int + int\$
int \$	int + int\$
\$	+ int\$

	int	()	+	*
E	1	2			
Op				3	4

LL(1) Error Detection, Part II

- (1) **E** \rightarrow **int**
- (2) **E** \rightarrow (**E Op E**)
- (3) **Op** \rightarrow **+**
- (4) **Op** \rightarrow *****

(int (int))\$

	int	()	+	*
E	1	2			
Op				3	4

LL(1) Error Detection, Part II

- (1) $E \rightarrow \text{int}$
- (2) $E \rightarrow (E \text{ Op } E)$
- (3) $\text{Op} \rightarrow +$
- (4) $\text{Op} \rightarrow *$

E\$	(int (int))\$
-----	---------------

	int	()	+	*
E	1	2			
Op				3	4

LL(1) Error Detection, Part II

- (1) $E \rightarrow \text{int}$
- (2) $E \rightarrow (E \text{ Op } E)$
- (3) $\text{Op} \rightarrow +$
- (4) $\text{Op} \rightarrow *$

E\$	(int (int))\$
-----	---------------

	int	()	+	*
E	1	2			
Op				3	4

LL(1) Error Detection, Part II

- (1) $E \rightarrow \text{int}$
- (2) $E \rightarrow (E \text{ Op } E)$
- (3) $\text{Op} \rightarrow +$
- (4) $\text{Op} \rightarrow *$

$E\$$	$(\text{int } (\text{int}))\$$
$(E \text{ Op } E) \$$	$(\text{int } (\text{int}))\$$

	int	()	+	*
E	1	2			
Op				3	4

LL(1) Error Detection, Part II

- (1) **E** \rightarrow **int**
- (2) **E** \rightarrow **(E Op E)**
- (3) **Op** \rightarrow **+**
- (4) **Op** \rightarrow *****

E\$	(int (int))\$
(E Op E) \$	(int (int))\$
E Op E) \$	int (int))\$

	int	()	+	*
E	1	2			
Op				3	4

LL(1) Error Detection, Part II

- (1) **E** \rightarrow **int**
- (2) **E** \rightarrow (**E Op E**)
- (3) **Op** \rightarrow **+**
- (4) **Op** \rightarrow *****

E\$	(int (int))\$
(E Op E) \$	(int (int))\$
E Op E) \$	int (int))\$

	int	()	+	*
E	1	2			
Op				3	4

LL(1) Error Detection, Part II

- (1) $E \rightarrow \text{int}$
 (2) $E \rightarrow (E \text{ Op } E)$
 (3) $\text{Op} \rightarrow +$
 (4) $\text{Op} \rightarrow *$

$E\$$	$(\text{int } (\text{int}))\$$
$(E \text{ Op } E) \$$	$(\text{int } (\text{int}))\$$
$E \text{ Op } E) \$$	$\text{int } (\text{int}))\$$
$\text{int Op } E) \$$	$\text{int } (\text{int}))\$$

	int	()	+	*
E	1	2			
Op				3	4

LL(1) Error Detection, Part II

- (1) $E \rightarrow \text{int}$
- (2) $E \rightarrow (E \text{ Op } E)$
- (3) $\text{Op} \rightarrow +$
- (4) $\text{Op} \rightarrow *$

$E\$$	$(\text{int } (\text{int}))\$$
$(E \text{ Op } E) \$$	$(\text{int } (\text{int}))\$$
$E \text{ Op } E) \$$	$\text{int } (\text{int}))\$$
$\text{int } \text{Op } E) \$$	$\text{int } (\text{int}))\$$
$\text{Op } E) \$$	$(\text{int}))\$$

	int	()	+	*
E	1	2			
Op				3	4

LL(1) Error Detection, Part II

- (1) **E** \rightarrow **int**
 (2) **E** \rightarrow **(E Op E)**
 (3) **Op** \rightarrow **+**
 (4) **Op** \rightarrow *****

E\$	(int (int))\$
(E Op E) \$	(int (int))\$
E Op E) \$	int (int))\$
int Op E) \$	int (int))\$
Op E) \$	(int))\$

	int	()	+	*
E	1	2			
Op				3	4

The LL(1) Algorithm

- Suppose a grammar has start symbol **S** and LL(1) parsing table T. We want to parse string ω
- Initialize a stack containing **S** $\$$.
- Repeat until the stack is empty:
 - Let the next character of ω be **t**.
 - If the top of the stack is a terminal **r**:
 - If **r** and **t** don't match, report an error.
 - Otherwise consume the character **t** and pop **r** from the stack.
 - Otherwise, the top of the stack is a nonterminal **A**:
 - _ If T[**A**, **t**] is undefined, report an error.
 - _ Replace the top of the stack with T[**A**, **t**].

LL(1) Parse Tables

$E \rightarrow \text{int}$

$E \rightarrow (E \text{ Op } E)$

$\text{Op} \rightarrow +$

$\text{Op} \rightarrow *$

	int	()	+	*
E	int	(E Op E)			
Op				+	*